@prefix : <https://github.com/MattiaSpadoni/LastSupper/blob/main/LastSupper.owl#> .
@prefix owl: <http://www.w3.org/2002/07/owl#> .
@prefix rdf: <http://www.w3.org/1999/02/22-rdf-syntax-ns#> .
@prefix xml: <http://www.w3.org/XML/1998/namespace> .
@prefix xsd: <http://www.w3.org/2001/XMLSchema#> .
@prefix rdfs: <http://www.w3.org/2000/01/rdf-schema#> .
@base <https://github.com/MattiaSpadoni/LastSupper/blob/main/LastSupper.owl#> .

<https://github.com/MattiaSpadoni/LastSupper/blob/main/LastSupper.owl#> rdf:type owl:Ontology .

#################################################################
#    Object Properties
#################################################################

###  http://www.ontologydesignpatterns.org/ont/dul/DUL.owl/associatedWith
<http://www.ontologydesignpatterns.org/ont/dul/DUL.owl/associatedWith> rdf:type owl:ObjectProperty .


###  http://www.ontologydesignpatterns.org/ont/dul/DUL.owl/classifies
<http://www.ontologydesignpatterns.org/ont/dul/DUL.owl/classifies> rdf:type owl:ObjectProperty ;
                                                                   rdfs:subPropertyOf <http://www.ontologydesignpatterns.org/ont/dul/DUL.owl/associatedWith> ;
                                                                   owl:inverseOf <http://www.ontologydesignpatterns.org/ont/dul/DUL.owl/isClassifiedBy> .


###  http://www.ontologydesignpatterns.org/ont/dul/DUL.owl/hasSetting
<http://www.ontologydesignpatterns.org/ont/dul/DUL.owl/hasSetting> rdf:type owl:ObjectProperty ;
                                                                   rdfs:subPropertyOf <http://www.ontologydesignpatterns.org/ont/dul/DUL.owl/associatedWith> ;
                                                                   owl:inverseOf <http://www.ontologydesignpatterns.org/ont/dul/DUL.owl/isSettingFor> .


###  http://www.ontologydesignpatterns.org/ont/dul/DUL.owl/isClassifiedBy
<http://www.ontologydesignpatterns.org/ont/dul/DUL.owl/isClassifiedBy> rdf:type owl:ObjectProperty ;
                                                                       rdfs:subPropertyOf <http://www.ontologydesignpatterns.org/ont/dul/DUL.owl/associatedWith> .


###  http://www.ontologydesignpatterns.org/ont/dul/DUL.owl/isSettingFor
<http://www.ontologydesignpatterns.org/ont/dul/DUL.owl/isSettingFor> rdf:type owl:ObjectProperty ;
                                                                     rdfs:subPropertyOf <http://www.ontologydesignpatterns.org/ont/dul/DUL.owl/associatedWith> .


###  https://github.com/MattiaSpadoni/LastSupper/blob/main/LastSupper.owl#ArtisticTheoryEmbodiedIn
:ArtisticTheoryEmbodiedIn rdf:type owl:ObjectProperty ;
                          rdfs:subPropertyOf :IsPresentIn ;
                          owl:inverseOf :EmbodiesArtisticTheory ;
                          rdfs:domain :ArtisticTheory ;
                          rdfs:range [ rdf:type owl:Class ;
                                       owl:unionOf ( :AbstractConcept
                                                     <https://w3id.org/arco/ontology/arco/CulturalProperty>
                                                   )
                                     ] ;
                          rdfs:comment "This property link an Iconographical Representation to the Theory it embodies inside it. Da Vinci Last Supper Iconography embodies Theory of Moti dell'Animo inside it." .


###  https://github.com/MattiaSpadoni/LastSupper/blob/main/LastSupper.owl#BelongsTo
:BelongsTo rdf:type owl:ObjectProperty ;
           owl:inverseOf :IsCulturalScopeOf ;
           rdfs:domain :AbstractConcept ;
           rdfs:range <https://w3id.org/arco/ontology/context-description/hasCulturalScope> ;
           rdfs:comment "This property link and abstract concept to its origin movement. Example: Teoria dei moti dell'animo was formalised during Renaissance and belongs to it." .


###  https://github.com/MattiaSpadoni/LastSupper/blob/main/LastSupper.owl#CompriseIconography
:CompriseIconography rdf:type owl:ObjectProperty ;
                     owl:inverseOf :IconographyCompriseIn ;
                     rdfs:domain :IconographicTheme ;
                     rdfs:range :Iconography ;
                     rdfs:comment "This property link the Iconographic theme to all its known Iconographies. Example: Last Supper Iconographic theme comprises Florentine Last Supper, Da Vinci Last Supper, Nordic Last Supper ecc..." .


###  https://github.com/MattiaSpadoni/LastSupper/blob/main/LastSupper.owl#CreatedBy
:CreatedBy rdf:type owl:ObjectProperty ;
           rdfs:subPropertyOf :IntroductedBy ;
           owl:inverseOf :Creates ;
           rdf:type owl:AsymmetricProperty ;
           rdfs:domain :Iconography ;
           rdfs:range <https://w3id.org/italia/onto/l0/Agent> ;
           rdfs:comment "Inverse of creates." .


###  https://github.com/MattiaSpadoni/LastSupper/blob/main/LastSupper.owl#Creates
:Creates rdf:type owl:ObjectProperty ;
         rdfs:subPropertyOf :Introduce ;
         rdfs:domain <https://w3id.org/italia/onto/l0/Agent> ;
         rdfs:range :Iconography ;
         rdfs:comment "This property highlights the role of creator an Agent played in the creation of an iconography. Eg: Leonardo created his own Last Supper iconography." .


###  https://github.com/MattiaSpadoni/LastSupper/blob/main/LastSupper.owl#EmbodiesArtisticTheory
:EmbodiesArtisticTheory rdf:type owl:ObjectProperty ;
                        rdfs:subPropertyOf :Presents ;
                        rdfs:domain [ rdf:type owl:Class ;
                                      owl:unionOf ( :AbstractConcept
                                                    <https://w3id.org/arco/ontology/arco/CulturalProperty>
                                                  )
                                    ] ;
                        rdfs:range :ArtisticTheory ;
                        rdfs:comment "Inverse of ArtisticTheoryEmbodied. It highlights the influence of a precise artistic theory on a cultural property or an abstract concept. Eg: Teoria dei moti dell'animo is present in most of Leonardo's drawings and works." .


###  https://github.com/MattiaSpadoni/LastSupper/blob/main/LastSupper.owl#HasCharacter
:HasCharacter rdf:type owl:ObjectProperty ;
              rdfs:subPropertyOf :HasPictorialAttribute ;
              owl:inverseOf :IsCharacterOf ;
              rdfs:domain :Iconography ;
              rdfs:range :Character ;
              rdfs:comment "This property links an iconography to a character present inside it indipendently from its shape." .


###  https://github.com/MattiaSpadoni/LastSupper/blob/main/LastSupper.owl#HasCompositionMotif
:HasCompositionMotif rdf:type owl:ObjectProperty ;
                     rdfs:subPropertyOf :HasVisualUnit ;
                     owl:inverseOf :IsCompositionMotifOf ;
                     rdfs:domain owl:Thing ;
                     rdfs:range :CompositionMotif ;
                     rdfs:comment "This property links an owl:thing to a visual representation of its composition characteristics. This property was born from Panofsky first level of interpretation where motifs are the display and the organisation of elements in the scene without going further in the interpretation. Eg: In Last Supper the presence of all figures on the other side of the table is a CompositionMotif" .


###  https://github.com/MattiaSpadoni/LastSupper/blob/main/LastSupper.owl#HasDerivatedWork
:HasDerivatedWork rdf:type owl:ObjectProperty ;
                  rdfs:subPropertyOf <https://w3id.org/arco/ontology/context-description/isRelatedWorkSituationOf> ;
                  owl:inverseOf :IsDerivationIn ;
                  rdfs:domain :DerivationRelation ;
                  rdfs:range <https://w3id.org/arco/ontology/arco/CulturalProperty> ;
                  rdfs:comment "This property links the derivation work of the relation." .


###  https://github.com/MattiaSpadoni/LastSupper/blob/main/LastSupper.owl#HasDerivativeVisualUnit
:HasDerivativeVisualUnit rdf:type owl:ObjectProperty ;
                         rdfs:subPropertyOf :HasVisualUnit ;
                         owl:inverseOf :IsDerivatedVisualUnitOf ;
                         rdfs:domain :DerivationRelation ;
                         rdfs:range :VisualUnit ;
                         rdfs:comment "This property identifies the derivative visual element in a DerivationRelation." .


###  https://github.com/MattiaSpadoni/LastSupper/blob/main/LastSupper.owl#HasFinalVisualUnit
:HasFinalVisualUnit rdf:type owl:ObjectProperty ;
                    rdfs:subPropertyOf :HasVisualUnit ;
                    owl:inverseOf :IsFinalVisualUnitOf ;
                    rdfs:domain :PreparatoryRelation ;
                    rdfs:range :VisualUnit ;
                    rdfs:comment "Specialisation of VisualAtom. Identifying the Final Visual Atom of a Preparatory relation. Eg: in the relation between Windsor 12551 and Last Supper by Leonardo the final Visual Unit is the depiction of S. James on the fresco." .


###  https://github.com/MattiaSpadoni/LastSupper/blob/main/LastSupper.owl#HasFinalWork
:HasFinalWork rdf:type owl:ObjectProperty ;
              rdfs:subPropertyOf <https://w3id.org/arco/ontology/context-description/isRelatedWorkSituationOf> ;
              owl:inverseOf :IsFinalIn ;
              rdfs:domain :PreparatoryRelation ;
              rdfs:range <https://w3id.org/arco/ontology/arco/CulturalProperty> ;
              rdfs:comment "This property links a preparatory relation to the final work of the relation" .


###  https://github.com/MattiaSpadoni/LastSupper/blob/main/LastSupper.owl#HasGeometricVisualUnit
:HasGeometricVisualUnit rdf:type owl:ObjectProperty ;
                        rdfs:subPropertyOf :HasVisualUnit ;
                        owl:inverseOf :IsGeometricVisualUnitOf ;
                        rdfs:domain owl:Thing ;
                        rdfs:range :GeometricVisualUnit ;
                        rdfs:comment "This property links an owl:thing to a photo/representation with its geometrical elements. Eg: a photo with perspective lines of Leonardo's Last Supper." .


###  https://github.com/MattiaSpadoni/LastSupper/blob/main/LastSupper.owl#HasIconographicTheme
:HasIconographicTheme rdf:type owl:ObjectProperty ;
                      owl:inverseOf :RepresentSubject ;
                      rdfs:domain <https://w3id.org/arco/ontology/context-description/Subject> ;
                      rdfs:range :IconographicTheme ;
                      rdfs:comment "Inverse of RepresentSubject. It links a subject to its iconographic theme" .


###  https://github.com/MattiaSpadoni/LastSupper/blob/main/LastSupper.owl#HasIconography
:HasIconography rdf:type owl:ObjectProperty ;
                owl:inverseOf :IsUsedInWork ;
                rdfs:domain <https://w3id.org/arco/ontology/arco/CulturalProperty> ;
                rdfs:range :Iconography ;
                rdfs:comment "IsUsedInWork. It links a cultural property to the Iconography that it has inside it." .


###  https://github.com/MattiaSpadoni/LastSupper/blob/main/LastSupper.owl#HasInfluencedVisualUnit
:HasInfluencedVisualUnit rdf:type owl:ObjectProperty ;
                         rdfs:subPropertyOf :HasVisualUnit ;
                         owl:inverseOf :IsInfluencedVisualUnitOf ;
                         rdfs:domain :InfluenceRelation ;
                         rdfs:range :VisualUnit ;
                         rdfs:comment "This property link the visual element of the influenced work in a InfluenceRelation. In the relation between Leonardo's Last Supper and Giorgione's Le tre età, the last one is the influenced work. Its visual unit is the depiction of the young man." .


###  https://github.com/MattiaSpadoni/LastSupper/blob/main/LastSupper.owl#HasInfluencedWork
:HasInfluencedWork rdf:type owl:ObjectProperty ;
                   rdfs:subPropertyOf <https://w3id.org/arco/ontology/context-description/isRelatedWorkSituationOf> ;
                   owl:inverseOf :IsInfluencedIn ;
                   rdfs:domain :InfluenceRelation ;
                   rdfs:range <https://w3id.org/arco/ontology/arco/CulturalProperty> ;
                   rdfs:comment "This property links an influence relation to the cultural property being the influenced one of the relation." .


###  https://github.com/MattiaSpadoni/LastSupper/blob/main/LastSupper.owl#HasInfluencerVisualUnit
:HasInfluencerVisualUnit rdf:type owl:ObjectProperty ;
                         rdfs:subPropertyOf :HasVisualUnit ;
                         owl:inverseOf :IsInfluencerVisualUnitOf ;
                         rdfs:domain :InfluenceRelation ;
                         rdfs:range :VisualUnit ;
                         rdfs:comment "This property link the visual unit of the influencer in a InfluenceRelation. In the relation between Leonardo's Last Supper and Giorgione's Le tre età Last Supper is the influencer. Its Visual Unit is the depiction of S. Philip's figure." .


###  https://github.com/MattiaSpadoni/LastSupper/blob/main/LastSupper.owl#HasInfluencerWork
:HasInfluencerWork rdf:type owl:ObjectProperty ;
                   rdfs:subPropertyOf <https://w3id.org/arco/ontology/context-description/isRelatedWorkSituationOf> ;
                   owl:inverseOf :IsInfluencerIn ;
                   rdfs:domain :InfluenceRelation ;
                   rdfs:range <https://w3id.org/arco/ontology/arco/CulturalProperty> ;
                   rdfs:comment "This property links an influence Relation to the cultural property being the influencer." .


###  https://github.com/MattiaSpadoni/LastSupper/blob/main/LastSupper.owl#HasLocation
:HasLocation rdf:type owl:ObjectProperty ;
             owl:inverseOf :IsLocationOf ;
             rdfs:domain owl:Thing ;
             rdfs:range <https://w3id.org/italia/onto/l0/Location> ;
             rdfs:comment "This property links an owl:Thing to a particular location" .


###  https://github.com/MattiaSpadoni/LastSupper/blob/main/LastSupper.owl#HasMediumVisualUnit
:HasMediumVisualUnit rdf:type owl:ObjectProperty ;
                     rdfs:subPropertyOf :HasVisualUnit ;
                     owl:inverseOf :IsMediumVisualUnitOf ;
                     rdfs:domain :InfluenceRelation ;
                     rdfs:range :VisualUnit ;
                     rdfs:comment "This property link the medium visual element of an InfluenceRelation. In the case of Influence relation between Leonardo's Last Supper and Coecke's Last Supper, Birago's Last Supper played the role of medium among them. The visual Unit is the depiction of the elements allowing the establisment of this role." .


###  https://github.com/MattiaSpadoni/LastSupper/blob/main/LastSupper.owl#HasMediumWork
:HasMediumWork rdf:type owl:ObjectProperty ;
               rdfs:subPropertyOf <https://w3id.org/arco/ontology/context-description/isRelatedWorkSituationOf> ;
               owl:inverseOf :IsMediumIn ;
               rdfs:domain :InfluenceRelation ;
               rdfs:range <https://w3id.org/arco/ontology/arco/CulturalProperty> ;
               rdfs:comment "This property links the InfluenceRelation to the cultural property being the medium of influence in the relation." .


###  https://github.com/MattiaSpadoni/LastSupper/blob/main/LastSupper.owl#HasObject
:HasObject rdf:type owl:ObjectProperty ;
           rdfs:subPropertyOf :HasPictorialAttribute ;
           owl:inverseOf :IsObjectOf ;
           rdfs:domain :Iconography ;
           rdfs:range :SceneObject ;
           rdfs:comment "This property links an iconography to a certain object inside it. In this case it is not important the shape of the figure, but the presence of that specific element. Eg: in Last Supper S. Peter always has a knife indipendently from its shape." .


###  https://github.com/MattiaSpadoni/LastSupper/blob/main/LastSupper.owl#HasOriginalVisualUnit
:HasOriginalVisualUnit rdf:type owl:ObjectProperty ;
                       rdfs:subPropertyOf :HasVisualUnit ;
                       owl:inverseOf :IsOriginalVisualUnitOf ;
                       rdfs:domain :DerivationRelation ;
                       rdfs:range :VisualUnit ;
                       rdfs:comment "This property identifies the original visual element in a DerivationRelation." .


###  https://github.com/MattiaSpadoni/LastSupper/blob/main/LastSupper.owl#HasOriginalWork
:HasOriginalWork rdf:type owl:ObjectProperty ;
                 rdfs:subPropertyOf <https://w3id.org/arco/ontology/context-description/isRelatedWorkSituationOf> ;
                 owl:inverseOf :IsOriginaln ;
                 rdfs:domain :DerivationRelation ;
                 rdfs:range <https://w3id.org/arco/ontology/arco/CulturalProperty> ;
                 rdfs:comment "This property links the Derivation Relation to the cultural property be the original one in the relation." .


###  https://github.com/MattiaSpadoni/LastSupper/blob/main/LastSupper.owl#HasPictorialAttribute
:HasPictorialAttribute rdf:type owl:ObjectProperty ;
                       owl:inverseOf :IsAttributeOf ;
                       rdfs:domain :Iconography ;
                       rdfs:range :PictorialAttribute ;
                       rdfs:comment "This property link an iconographical representation to a pictorial attribute part of it. eg: Last Supper has the figure of Christ inside it." .


###  https://github.com/MattiaSpadoni/LastSupper/blob/main/LastSupper.owl#HasPreparatoryVisualUnit
:HasPreparatoryVisualUnit rdf:type owl:ObjectProperty ;
                          rdfs:subPropertyOf :HasVisualUnit ;
                          owl:inverseOf :IsPreparatoryVisualUnitOf ;
                          rdfs:domain :PreparatoryRelation ;
                          rdfs:range :VisualUnit ;
                          rdfs:comment "This property highlights the preparatory visual element of a Preparatory Relation. Eg: in the relation between Windsor 12551 and Last Supper by Leonardo the preparatory Visual Unit is the depiction of S. James in the Windsor sheet." .


###  https://github.com/MattiaSpadoni/LastSupper/blob/main/LastSupper.owl#HasPreparatoryWork
:HasPreparatoryWork rdf:type owl:ObjectProperty ;
                    rdfs:subPropertyOf <https://w3id.org/arco/ontology/context-description/isRelatedWorkSituationOf> ;
                    owl:inverseOf :IsPreparatoryIn ;
                    rdfs:domain :PreparatoryRelation ;
                    rdfs:range <https://w3id.org/arco/ontology/arco/CulturalProperty> ;
                    rdfs:comment "This property link a preparatory relation to the cultural property being the preparatory work in the relation" .


###  https://github.com/MattiaSpadoni/LastSupper/blob/main/LastSupper.owl#HasVisualUnit
:HasVisualUnit rdf:type owl:ObjectProperty ;
               owl:inverseOf :IsVisualUnitOf ;
               rdfs:domain owl:Thing ;
               rdfs:range :VisualUnit ;
               rdfs:comment "Property linking an Owl:thing to a Visual Uni representing a significant visual feature of it. Eg: Da Vinci's Last Supper Iconography linked to a Visual Unit showing some visible feature of the iconography itself. The visual element is not meaningful by itself, but it is significant for its colors and shapes." .


###  https://github.com/MattiaSpadoni/LastSupper/blob/main/LastSupper.owl#IconographyCompriseIn
:IconographyCompriseIn rdf:type owl:ObjectProperty ;
                       rdfs:domain :Iconography ;
                       rdfs:range :IconographicTheme ;
                       rdfs:comment "Inverse of CompriseIconography" .


###  https://github.com/MattiaSpadoni/LastSupper/blob/main/LastSupper.owl#Influenced
:Influenced rdf:type owl:ObjectProperty ;
            owl:inverseOf :InfluencedBy ;
            rdfs:domain :ArtisticTheory ;
            rdfs:range :Iconography ;
            rdfs:comment "This property highlights the influence that an artistic Theory has on an iconographies." .


###  https://github.com/MattiaSpadoni/LastSupper/blob/main/LastSupper.owl#InfluencedBy
:InfluencedBy rdf:type owl:ObjectProperty ;
              rdfs:domain :Iconography ;
              rdfs:range :ArtisticTheory ;
              rdfs:comment "Inverse of Influenced." .


###  https://github.com/MattiaSpadoni/LastSupper/blob/main/LastSupper.owl#Introduce
:Introduce rdf:type owl:ObjectProperty ;
           owl:inverseOf :IntroductedBy ;
           rdfs:domain <https://w3id.org/italia/onto/l0/Agent> ;
           rdfs:range :AbstractConcept ;
           rdfs:comment "Inverse of IntroducedBy. This property highlight the role of creator an Agent played in the birth of an abstract concept" .


###  https://github.com/MattiaSpadoni/LastSupper/blob/main/LastSupper.owl#IntroductedBy
:IntroductedBy rdf:type owl:ObjectProperty ;
               rdfs:domain :AbstractConcept ;
               rdfs:range <https://w3id.org/italia/onto/l0/Agent> ;
               rdfs:comment "Inverse of Introduce." .


###  https://github.com/MattiaSpadoni/LastSupper/blob/main/LastSupper.owl#IsAttributeOf
:IsAttributeOf rdf:type owl:ObjectProperty ;
               rdfs:domain :PictorialAttribute ;
               rdfs:range :Iconography ;
               rdfs:comment "Inverse of  HasAttribute" .


###  https://github.com/MattiaSpadoni/LastSupper/blob/main/LastSupper.owl#IsCharacterOf
:IsCharacterOf rdf:type owl:ObjectProperty ;
               rdfs:subPropertyOf :IsAttributeOf ;
               rdfs:domain :Character ;
               rdfs:range :Iconography ;
               rdfs:comment "Inverse of HasCharacter." .


###  https://github.com/MattiaSpadoni/LastSupper/blob/main/LastSupper.owl#IsCompositionMotifOf
:IsCompositionMotifOf rdf:type owl:ObjectProperty ;
                      rdfs:subPropertyOf :IsVisualUnitOf ;
                      rdfs:domain :CompositionMotif ;
                      rdfs:range owl:Thing ;
                      rdfs:comment "Inverse of HasCompositionMotif." .


###  https://github.com/MattiaSpadoni/LastSupper/blob/main/LastSupper.owl#IsCulturalScopeOf
:IsCulturalScopeOf rdf:type owl:ObjectProperty ;
                   rdfs:domain <https://w3id.org/arco/ontology/context-description/hasCulturalScope> ;
                   rdfs:range :AbstractConcept ;
                   rdfs:comment "Inverse of BelongsTo" .


###  https://github.com/MattiaSpadoni/LastSupper/blob/main/LastSupper.owl#IsDerivatedVisualUnitOf
:IsDerivatedVisualUnitOf rdf:type owl:ObjectProperty ;
                         rdfs:subPropertyOf :IsVisualUnitOf ;
                         rdfs:domain :VisualUnit ;
                         rdfs:range :DerivationRelation ;
                         rdfs:comment "Inverse of HasDerivativeVisualUnit." .


###  https://github.com/MattiaSpadoni/LastSupper/blob/main/LastSupper.owl#IsDerivationIn
:IsDerivationIn rdf:type owl:ObjectProperty ;
                rdfs:subPropertyOf <https://w3id.org/arco/ontology/context-description/hasRelatedWorkSituation> ;
                rdfs:domain <https://w3id.org/arco/ontology/arco/CulturalProperty> ;
                rdfs:range :DerivationRelation ;
                rdfs:comment "This property link a cultural Property to the DerivationRelation node. Specifically this property link the derivation one of the 2 Cultural Properties." .


###  https://github.com/MattiaSpadoni/LastSupper/blob/main/LastSupper.owl#IsFinalIn
:IsFinalIn rdf:type owl:ObjectProperty ;
           rdfs:subPropertyOf <https://w3id.org/arco/ontology/context-description/hasRelatedWorkSituation> ;
           rdfs:domain <https://w3id.org/arco/ontology/arco/CulturalProperty> ;
           rdfs:range :PreparatoryRelation ;
           rdfs:comment "This property link a Cultural Property to its PreparatoryRelation node. Specifically this property identify the final work of the relation." .


###  https://github.com/MattiaSpadoni/LastSupper/blob/main/LastSupper.owl#IsFinalVisualUnitOf
:IsFinalVisualUnitOf rdf:type owl:ObjectProperty ;
                     rdfs:subPropertyOf :IsVisualUnitOf ;
                     rdfs:domain :VisualUnit ;
                     rdfs:range :PreparatoryRelation ;
                     rdfs:comment "Inverse of HasFinalVisualUnit" .


###  https://github.com/MattiaSpadoni/LastSupper/blob/main/LastSupper.owl#IsGeometricVisualUnitOf
:IsGeometricVisualUnitOf rdf:type owl:ObjectProperty ;
                         rdfs:subPropertyOf :IsVisualUnitOf ;
                         rdfs:domain :GeometricVisualUnit ;
                         rdfs:range owl:Thing ;
                         rdfs:comment "Inverse of HasGeometricVisualUnit" .


###  https://github.com/MattiaSpadoni/LastSupper/blob/main/LastSupper.owl#IsInfluencedIn
:IsInfluencedIn rdf:type owl:ObjectProperty ;
                rdfs:subPropertyOf <https://w3id.org/arco/ontology/context-description/hasRelatedWorkSituation> ;
                rdfs:domain <https://w3id.org/arco/ontology/arco/CulturalProperty> ;
                rdfs:range :InfluenceRelation ;
                rdfs:comment "This property links a Cultural Property to its influence relation node. Specifically this property identify the cultural property that is influenced by another one." .


###  https://github.com/MattiaSpadoni/LastSupper/blob/main/LastSupper.owl#IsInfluencedVisualUnitOf
:IsInfluencedVisualUnitOf rdf:type owl:ObjectProperty ;
                          rdfs:subPropertyOf :IsVisualUnitOf ;
                          rdfs:domain :VisualUnit ;
                          rdfs:range :InfluenceRelation ;
                          rdfs:comment "Inverse of HasInfluencedVisualUnit" .


###  https://github.com/MattiaSpadoni/LastSupper/blob/main/LastSupper.owl#IsInfluencerIn
:IsInfluencerIn rdf:type owl:ObjectProperty ;
                rdfs:subPropertyOf <https://w3id.org/arco/ontology/context-description/hasRelatedWorkSituation> ;
                rdfs:domain <https://w3id.org/arco/ontology/arco/CulturalProperty> ;
                rdfs:range :InfluenceRelation ;
                rdfs:comment "This property links a Cultural Property to its influence relation node. Specifically this property identify the cultural property that influence the other one." .


###  https://github.com/MattiaSpadoni/LastSupper/blob/main/LastSupper.owl#IsInfluencerVisualUnitOf
:IsInfluencerVisualUnitOf rdf:type owl:ObjectProperty ;
                          rdfs:subPropertyOf :IsVisualUnitOf ;
                          rdfs:domain :VisualUnit ;
                          rdfs:range :InfluenceRelation ;
                          rdfs:comment "Inverse of HasInfluencerVisualUnit." .


###  https://github.com/MattiaSpadoni/LastSupper/blob/main/LastSupper.owl#IsLocationOf
:IsLocationOf rdf:type owl:ObjectProperty ;
              rdfs:domain <https://w3id.org/italia/onto/l0/Location> ;
              rdfs:range owl:Thing ;
              rdfs:comment "Inverse of HasLocation." .


###  https://github.com/MattiaSpadoni/LastSupper/blob/main/LastSupper.owl#IsMediumIn
:IsMediumIn rdf:type owl:ObjectProperty ;
            rdfs:subPropertyOf <https://w3id.org/arco/ontology/context-description/hasRelatedWorkSituation> ;
            rdfs:comment "This property highlights the role of medium in the relation between 2 cultural properties. Eg: The incision from Pietro Birago of Last Supper was the medium of influence from Last Supper to the Flanders." .


###  https://github.com/MattiaSpadoni/LastSupper/blob/main/LastSupper.owl#IsMediumVisualUnitOf
:IsMediumVisualUnitOf rdf:type owl:ObjectProperty ;
                      rdfs:subPropertyOf :IsVisualUnitOf ;
                      rdfs:domain :VisualUnit ;
                      rdfs:range :InfluenceRelation ;
                      rdfs:comment "Inverse of HasMediumVisualUnit." .


###  https://github.com/MattiaSpadoni/LastSupper/blob/main/LastSupper.owl#IsObjectOf
:IsObjectOf rdf:type owl:ObjectProperty ;
            rdfs:subPropertyOf :IsAttributeOf ;
            rdfs:domain :SceneObject ;
            rdfs:range :Iconography ;
            rdfs:comment "Inverse of HasObject." .


###  https://github.com/MattiaSpadoni/LastSupper/blob/main/LastSupper.owl#IsOriginalVisualUnitOf
:IsOriginalVisualUnitOf rdf:type owl:ObjectProperty ;
                        rdfs:subPropertyOf :IsVisualUnitOf ;
                        rdfs:domain :VisualUnit ;
                        rdfs:range :DerivationRelation ;
                        rdfs:comment "Inverse of HasOriginalVisualUnit." .


###  https://github.com/MattiaSpadoni/LastSupper/blob/main/LastSupper.owl#IsOriginaln
:IsOriginaln rdf:type owl:ObjectProperty ;
             rdfs:subPropertyOf <https://w3id.org/arco/ontology/context-description/hasRelatedWorkSituation> ;
             rdfs:domain <https://w3id.org/arco/ontology/arco/CulturalProperty> ;
             rdfs:range :DerivationRelation ;
             rdfs:comment "This property links a cultural property to a derivation relation where it is the original work." .


###  https://github.com/MattiaSpadoni/LastSupper/blob/main/LastSupper.owl#IsPredecessorOf
:IsPredecessorOf rdf:type owl:ObjectProperty ;
                 owl:inverseOf :IsSuccessorOf ;
                 rdfs:domain :Iconography ;
                 rdfs:range :Iconography ;
                 rdfs:comment "This property link an iconographical representation to another one that come immediately before it. Eg: The Florentine iconographical representation is the predecessor of Da Vinci's one." .


###  https://github.com/MattiaSpadoni/LastSupper/blob/main/LastSupper.owl#IsPreparatoryIn
:IsPreparatoryIn rdf:type owl:ObjectProperty ;
                 rdfs:subPropertyOf <https://w3id.org/arco/ontology/context-description/hasRelatedWorkSituation> ;
                 rdfs:domain <https://w3id.org/arco/ontology/arco/CulturalProperty> ;
                 rdfs:range :PreparatoryRelation ;
                 rdfs:comment "This property links a cultural property to a relation where it is a preparatory work." .


###  https://github.com/MattiaSpadoni/LastSupper/blob/main/LastSupper.owl#IsPreparatoryVisualUnitOf
:IsPreparatoryVisualUnitOf rdf:type owl:ObjectProperty ;
                           rdfs:subPropertyOf :IsVisualUnitOf ;
                           rdfs:domain :VisualUnit ;
                           rdfs:range :PreparatoryRelation ;
                           rdfs:comment "Inverse of HasPreparatoryVisualUnit" .


###  https://github.com/MattiaSpadoni/LastSupper/blob/main/LastSupper.owl#IsPresentIn
:IsPresentIn rdf:type owl:ObjectProperty ;
             owl:inverseOf :Presents ;
             rdfs:domain :AbstractConcept ;
             rdfs:range [ rdf:type owl:Class ;
                          owl:unionOf ( :AbstractConcept
                                        <https://w3id.org/arco/ontology/arco/CulturalProperty>
                                      )
                        ] ;
             rdfs:comment "It highlights the presence of an abstract concept inside a Cultural property. Eg: Da Vinci's iconographical rapresentation of Last Supper is present in a set of different Cultural Properties. Teoria dei Moti dell'animo is present in another set of other Cultural Properties." .


###  https://github.com/MattiaSpadoni/LastSupper/blob/main/LastSupper.owl#IsRelationLocationOf
:IsRelationLocationOf rdf:type owl:ObjectProperty ;
                      rdfs:subPropertyOf :IsLocationOf ;
                      owl:inverseOf :hasRelationLocation ;
                      rdfs:domain <https://w3id.org/italia/onto/l0/Location> ;
                      rdfs:range <https://w3id.org/arco/ontology/context-description/RelatedWorkSituation> ;
                      rdfs:comment "Inverse of HasRelationLocation" .


###  https://github.com/MattiaSpadoni/LastSupper/blob/main/LastSupper.owl#IsStartingLocationOf
:IsStartingLocationOf rdf:type owl:ObjectProperty ;
                      rdfs:subPropertyOf :IsLocationOf ;
                      owl:inverseOf :hasStartingLocation ;
                      rdfs:domain <https://w3id.org/italia/onto/l0/Location> ;
                      rdfs:range :AbstractConcept ;
                      rdfs:comment "Inverse of HasStartingLocation" .


###  https://github.com/MattiaSpadoni/LastSupper/blob/main/LastSupper.owl#IsSuccessorOf
:IsSuccessorOf rdf:type owl:ObjectProperty ;
               rdfs:subPropertyOf owl:topObjectProperty ;
               rdfs:domain :Iconography ;
               rdfs:range :Iconography ;
               rdfs:comment "Inverse of IsPredecessorOf. It links an iconography to a successive one. Eg. Late Florentine Last Supper Iconography is successor of Early Florentine Last Supper Iconography." .


###  https://github.com/MattiaSpadoni/LastSupper/blob/main/LastSupper.owl#IsUsedInWork
:IsUsedInWork rdf:type owl:ObjectProperty ;
              rdfs:domain :Iconography ;
              rdfs:range <https://w3id.org/arco/ontology/arco/CulturalProperty> ;
              rdfs:comment "Inverse of HasIconography" .


###  https://github.com/MattiaSpadoni/LastSupper/blob/main/LastSupper.owl#IsVisualUnitOf
:IsVisualUnitOf rdf:type owl:ObjectProperty ;
                rdfs:domain :VisualUnit ;
                rdfs:range owl:Thing ;
                rdfs:comment "Inverse of HasVisualUnit." .


###  https://github.com/MattiaSpadoni/LastSupper/blob/main/LastSupper.owl#Presents
:Presents rdf:type owl:ObjectProperty ;
          rdfs:domain [ rdf:type owl:Class ;
                        owl:unionOf ( :AbstractConcept
                                      <https://w3id.org/arco/ontology/arco/CulturalProperty>
                                    )
                      ] ;
          rdfs:range :AbstractConcept ;
          rdfs:comment "Inverse of IsPresentIn. This property means that an abstract concept or a cultural property show characteristics of another abstract concept." .


###  https://github.com/MattiaSpadoni/LastSupper/blob/main/LastSupper.owl#RepresentSubject
:RepresentSubject rdf:type owl:ObjectProperty ;
                  rdfs:domain :IconographicTheme ;
                  rdfs:range <https://w3id.org/arco/ontology/context-description/Subject> ;
                  rdfs:comment "This property link an iconographic theme to its a-cd:Subject. Eg: Last Supper iconographic theme represent the a-cd:subject \"Last Supper\" or \"Cena Domini\"." .


###  https://github.com/MattiaSpadoni/LastSupper/blob/main/LastSupper.owl#TheorisedBy
:TheorisedBy rdf:type owl:ObjectProperty ;
             rdfs:subPropertyOf :IntroductedBy ;
             owl:inverseOf :Theorises ;
             rdfs:domain :ArtisticTheory ;
             rdfs:range <https://w3id.org/italia/onto/l0/Agent> ;
             rdfs:comment "Inverse of Theorises" .


###  https://github.com/MattiaSpadoni/LastSupper/blob/main/LastSupper.owl#Theorises
:Theorises rdf:type owl:ObjectProperty ;
           rdfs:subPropertyOf :Introduce ;
           rdfs:domain <https://w3id.org/italia/onto/l0/Agent> ;
           rdfs:range :ArtisticTheory ;
           rdfs:comment "This property highlights the role of theoriser an Agent played for an artistic theory. It does not necessarily imply the agent to be a conscious theoriser. Leonardo is one of the theorisers of Teoria dei Moti dell'Animo even though he did not that on purpose." .


###  https://github.com/MattiaSpadoni/LastSupper/blob/main/LastSupper.owl#hasDepiction
:hasDepiction rdf:type owl:ObjectProperty ;
              rdfs:subPropertyOf <https://w3id.org/arco/ontology/context-description/hasDepiction> ;
              rdfs:domain [ rdf:type owl:Class ;
                            owl:unionOf ( <http://dati.beniculturali.it/cis/CulturalEntity>
                                          :VisualUnit
                                          <https://w3id.org/italia/onto/l0/Agent>
                                        )
                          ] ;
              rdfs:range <http://xmlns.com/foaf/0.1/Image> ;
              rdfs:comment "This property relates an entity to its depiction." .


###  https://github.com/MattiaSpadoni/LastSupper/blob/main/LastSupper.owl#hasDiffusionPeriod
:hasDiffusionPeriod rdf:type owl:ObjectProperty ;
                    rdfs:domain :AbstractConcept ;
                    rdfs:range <https://w3id.org/italia/onto/TI/TimeInterval> ;
                    rdfs:comment "This property links an abstract concept to its diffusion time period." .


###  https://github.com/MattiaSpadoni/LastSupper/blob/main/LastSupper.owl#hasRelationLocation
:hasRelationLocation rdf:type owl:ObjectProperty ;
                     rdfs:subPropertyOf :HasLocation ;
                     rdfs:domain <https://w3id.org/arco/ontology/context-description/RelatedWorkSituation> ;
                     rdfs:range <https://w3id.org/italia/onto/l0/Location> ;
                     rdfs:comment "This property links a relation to the place where it happened (if it is known)." .


###  https://github.com/MattiaSpadoni/LastSupper/blob/main/LastSupper.owl#hasStartingLocation
:hasStartingLocation rdf:type owl:ObjectProperty ;
                     rdfs:subPropertyOf :HasLocation ;
                     rdfs:domain :AbstractConcept ;
                     rdfs:range <https://w3id.org/italia/onto/l0/Location> ;
                     rdfs:comment "This property links an abstract concept to the place where it started (if it is known). Eg: Leonardo's Last Supper iconography started in Milan" .


###  https://w3id.org/arco/ontology/context-description/hasAuthor
<https://w3id.org/arco/ontology/context-description/hasAuthor> rdf:type owl:ObjectProperty ;
                                                               rdfs:subPropertyOf <https://w3id.org/arco/ontology/context-description/hasRelatedAgent> ;
                                                               owl:inverseOf <https://w3id.org/arco/ontology/context-description/isAuthorOf> ;
                                                               rdfs:domain owl:Thing ;
                                                               rdfs:range <https://w3id.org/italia/onto/l0/Agent> ;
                                                               rdfs:comment """This property relates an entity to its author.
This property relates a entity (i.e. documentation, cultural entity, etc.) to its author.""" .


###  https://w3id.org/arco/ontology/context-description/hasBibliography
<https://w3id.org/arco/ontology/context-description/hasBibliography> rdf:type owl:ObjectProperty ;
                                                                     owl:inverseOf <https://w3id.org/arco/ontology/context-description/isBibliographyOf> ;
                                                                     rdfs:domain owl:Thing ;
                                                                     rdfs:range <https://w3id.org/arco/ontology/context-description/Bibliography> ;
                                                                     rdfs:comment "This property relates an entity to its bibliography." .


###  https://w3id.org/arco/ontology/context-description/hasBibliographyType
<https://w3id.org/arco/ontology/context-description/hasBibliographyType> rdf:type owl:ObjectProperty ;
                                                                         rdfs:subPropertyOf <https://w3id.org/arco/ontology/core/hasType> ;
                                                                         owl:inverseOf <https://w3id.org/arco/ontology/context-description/isBibliographyTypeOf> ;
                                                                         rdfs:domain <https://w3id.org/arco/ontology/context-description/Bibliography> ;
                                                                         rdfs:range <https://w3id.org/arco/ontology/context-description/BibliographyType> .


###  https://w3id.org/arco/ontology/context-description/hasDating
<https://w3id.org/arco/ontology/context-description/hasDating> rdf:type owl:ObjectProperty ;
                                                               rdfs:subPropertyOf <https://w3id.org/arco/ontology/core/hasSituation> ;
                                                               owl:inverseOf <https://w3id.org/arco/ontology/context-description/isDatingOf> ;
                                                               rdfs:domain owl:Thing ;
                                                               rdfs:range <https://w3id.org/arco/ontology/context-description/Dating> ;
                                                               rdfs:comment "This property relates an entity to its dating." .


###  https://w3id.org/arco/ontology/context-description/hasDatingEvent
<https://w3id.org/arco/ontology/context-description/hasDatingEvent> rdf:type owl:ObjectProperty ;
                                                                    owl:inverseOf <https://w3id.org/arco/ontology/context-description/isDatingEventOf> ;
                                                                    rdfs:domain <https://w3id.org/arco/ontology/context-description/Dating> ;
                                                                    rdfs:range <https://w3id.org/italia/onto/l0/EventOrSituation> ;
                                                                    rdfs:comment "This property link the Dating node to its dating Event. The dating pattern is mutuated by the contextual description module." .


###  https://w3id.org/arco/ontology/context-description/hasDepiction
<https://w3id.org/arco/ontology/context-description/hasDepiction> rdf:type owl:ObjectProperty ;
                                                                  rdfs:comment "This property relates an entity to its depiction." .


###  https://w3id.org/arco/ontology/context-description/hasRelatedAgent
<https://w3id.org/arco/ontology/context-description/hasRelatedAgent> rdf:type owl:ObjectProperty ;
                                                                     owl:inverseOf <https://w3id.org/arco/ontology/context-description/isAgentRelatedTo> ;
                                                                     rdfs:domain owl:Thing ;
                                                                     rdfs:range <https://w3id.org/italia/onto/l0/Agent> ;
                                                                     rdfs:comment "This property is used to associate an entity of any kind to an agent related to that entity in some way. It is used when it is not possible to express the relation in a more specific way." .


###  https://w3id.org/arco/ontology/context-description/hasRelatedWorkSituation
<https://w3id.org/arco/ontology/context-description/hasRelatedWorkSituation> rdf:type owl:ObjectProperty ;
                                                                             rdfs:subPropertyOf <https://w3id.org/arco/ontology/core/hasSituation> ;
                                                                             owl:inverseOf <https://w3id.org/arco/ontology/context-description/isRelatedWorkSituationOf> ;
                                                                             rdfs:domain <https://w3id.org/arco/ontology/arco/CulturalProperty> ;
                                                                             rdfs:range <https://w3id.org/arco/ontology/context-description/RelatedWorkSituation> ;
                                                                             rdfs:comment "This property relates a cultural property to a situation in which this cultural property is related to another work, that could even be another cultural property, as its preparatory or final phase." .


###  https://w3id.org/arco/ontology/context-description/isAgentRelatedTo
<https://w3id.org/arco/ontology/context-description/isAgentRelatedTo> rdf:type owl:ObjectProperty ;
                                                                      rdfs:domain <https://w3id.org/italia/onto/l0/Agent> ;
                                                                      rdfs:range owl:Thing ;
                                                                      rdfs:comment "This property is used to associate an agent related in some way to an entity of any kind to that entity. It is used when it is not possible to express the relation in a more specific way." .


###  https://w3id.org/arco/ontology/context-description/isAuthorOf
<https://w3id.org/arco/ontology/context-description/isAuthorOf> rdf:type owl:ObjectProperty ;
                                                                rdfs:subPropertyOf <https://w3id.org/arco/ontology/context-description/isAgentRelatedTo> ;
                                                                rdfs:domain <https://w3id.org/italia/onto/l0/Agent> ;
                                                                rdfs:range owl:Thing ;
                                                                rdfs:comment "This property relates an agent to an entity the agent is author of." .


###  https://w3id.org/arco/ontology/context-description/isBibliographyOf
<https://w3id.org/arco/ontology/context-description/isBibliographyOf> rdf:type owl:ObjectProperty ;
                                                                      rdfs:subPropertyOf owl:topObjectProperty ;
                                                                      rdfs:domain <https://w3id.org/arco/ontology/context-description/Bibliography> ;
                                                                      rdfs:range owl:Thing ;
                                                                      rdfs:comment "This property relates a bibliography to the entity which is referred to." .


###  https://w3id.org/arco/ontology/context-description/isBibliographyTypeOf
<https://w3id.org/arco/ontology/context-description/isBibliographyTypeOf> rdf:type owl:ObjectProperty ;
                                                                          rdfs:subPropertyOf <https://w3id.org/arco/ontology/core/isTypeOf> ;
                                                                          rdfs:domain <https://w3id.org/arco/ontology/context-description/BibliographyType> ;
                                                                          rdfs:range <https://w3id.org/arco/ontology/context-description/Bibliography> ;
                                                                          rdfs:comment "This property relates the bibliography type to its bibliography." .


###  https://w3id.org/arco/ontology/context-description/isDatingEventOf
<https://w3id.org/arco/ontology/context-description/isDatingEventOf> rdf:type owl:ObjectProperty ;
                                                                     rdfs:domain <https://w3id.org/italia/onto/l0/EventOrSituation> ;
                                                                     rdfs:range <https://w3id.org/arco/ontology/context-description/Dating> ;
                                                                     rdfs:comment "This property relates an event involving the cultural property, which the dating is about, to a dating." .


###  https://w3id.org/arco/ontology/context-description/isDatingOf
<https://w3id.org/arco/ontology/context-description/isDatingOf> rdf:type owl:ObjectProperty ;
                                                                rdfs:subPropertyOf <https://w3id.org/arco/ontology/core/isSituationOf> ;
                                                                rdfs:domain <https://w3id.org/arco/ontology/context-description/Dating> ;
                                                                rdfs:range owl:Thing ;
                                                                rdfs:comment "This property relates a dating to an entity." .


###  https://w3id.org/arco/ontology/context-description/isRelatedWorkSituationOf
<https://w3id.org/arco/ontology/context-description/isRelatedWorkSituationOf> rdf:type owl:ObjectProperty ;
                                                                              rdfs:domain <https://w3id.org/arco/ontology/context-description/RelatedWorkSituation> ;
                                                                              rdfs:range <https://w3id.org/arco/ontology/arco/CulturalProperty> ;
                                                                              rdfs:comment "This property, inverse of 'has related work situation', relates a situation in which a cultural property is related to another work, that could even be another cultural property, to the cultural property." .


###  https://w3id.org/arco/ontology/context-description/specificTime
<https://w3id.org/arco/ontology/context-description/specificTime> rdf:type owl:ObjectProperty ;
                                                                  rdfs:subPropertyOf <https://w3id.org/italia/onto/TI/atTime> ;
                                                                  rdfs:domain <https://w3id.org/italia/onto/l0/EventOrSituation> ;
                                                                  rdfs:range <https://w3id.org/italia/onto/TI/TimeInterval> ;
                                                                  rdfs:comment "This property relates the event (creation, distruction) to which a dating of a cultural property is related to the \"specific time\", as the dating expressed in year or as a date yyyy/mm/dd." .


###  https://w3id.org/arco/ontology/core/hasConcept
<https://w3id.org/arco/ontology/core/hasConcept> rdf:type owl:ObjectProperty ;
                                                 rdfs:subPropertyOf <http://www.ontologydesignpatterns.org/ont/dul/DUL.owl/isClassifiedBy> ;
                                                 owl:inverseOf <https://w3id.org/arco/ontology/core/isConceptOf> .


###  https://w3id.org/arco/ontology/core/hasSituation
<https://w3id.org/arco/ontology/core/hasSituation> rdf:type owl:ObjectProperty ;
                                                   rdfs:subPropertyOf <http://www.ontologydesignpatterns.org/ont/dul/DUL.owl/hasSetting> ;
                                                   owl:inverseOf <https://w3id.org/arco/ontology/core/isSituationOf> ;
                                                   rdfs:comment "The property that links any object to a situation." .


###  https://w3id.org/arco/ontology/core/hasType
<https://w3id.org/arco/ontology/core/hasType> rdf:type owl:ObjectProperty ;
                                              rdfs:subPropertyOf <https://w3id.org/arco/ontology/core/hasConcept> ;
                                              owl:inverseOf <https://w3id.org/arco/ontology/core/isTypeOf> .


###  https://w3id.org/arco/ontology/core/isConceptOf
<https://w3id.org/arco/ontology/core/isConceptOf> rdf:type owl:ObjectProperty ;
                                                  rdfs:subPropertyOf <http://www.ontologydesignpatterns.org/ont/dul/DUL.owl/classifies> ;
                                                  rdfs:domain <https://w3id.org/italia/onto/l0/Concept> ;
                                                  rdfs:range owl:Thing ;
                                                  rdfs:comment "The inverse property of hasConcept, that relates a concept to any object." .


###  https://w3id.org/arco/ontology/core/isSituationOf
<https://w3id.org/arco/ontology/core/isSituationOf> rdf:type owl:ObjectProperty ;
                                                    rdfs:subPropertyOf <http://www.ontologydesignpatterns.org/ont/dul/DUL.owl/isSettingFor> .


###  https://w3id.org/arco/ontology/core/isTypeOf
<https://w3id.org/arco/ontology/core/isTypeOf> rdf:type owl:ObjectProperty ;
                                               rdfs:subPropertyOf <https://w3id.org/arco/ontology/core/isConceptOf> .


###  https://w3id.org/italia/onto/CLV/hasGeometry
<https://w3id.org/italia/onto/CLV/hasGeometry> rdf:type owl:ObjectProperty ;
                                               owl:inverseOf <https://w3id.org/italia/onto/CLV/isGeometryFor> ;
                                               rdfs:domain owl:Thing ;
                                               rdfs:range <https://w3id.org/italia/onto/CLV/Geometry> ;
                                               rdfs:comment "This property links any thing of the domain to the geometry." .


###  https://w3id.org/italia/onto/CLV/isGeometryFor
<https://w3id.org/italia/onto/CLV/isGeometryFor> rdf:type owl:ObjectProperty ;
                                                 rdfs:domain <https://w3id.org/italia/onto/CLV/Geometry> ;
                                                 rdfs:range owl:Thing ;
                                                 rdfs:comment "Inverse property of \"hasGeometry\" that links a geometry to the related Thing of the domain." .


###  https://w3id.org/italia/onto/TI/atTime
<https://w3id.org/italia/onto/TI/atTime> rdf:type owl:ObjectProperty ;
                                         rdfs:subPropertyOf <https://w3id.org/italia/onto/TI/hasTemporalEntity> ;
                                         rdfs:domain owl:Thing ;
                                         rdfs:range <https://w3id.org/italia/onto/TI/TimeInterval> ;
                                         rdfs:comment "Relation between any thing and time interval" .


###  https://w3id.org/italia/onto/TI/hasTemporalEntity
<https://w3id.org/italia/onto/TI/hasTemporalEntity> rdf:type owl:ObjectProperty ;
                                                    rdfs:domain owl:Thing ;
                                                    rdfs:range <https://w3id.org/italia/onto/TI/TemporalEntity> ;
                                                    rdfs:comment "Property that links a time indexed event to a temporal entity." .


#################################################################
#    Data properties
#################################################################

###  https://github.com/MattiaSpadoni/LastSupper/blob/main/LastSupper.owl#AlternativeRelationDate
:AlternativeRelationDate rdf:type owl:DatatypeProperty ;
                         rdfs:subPropertyOf <https://w3id.org/italia/onto/TI/date> ;
                         rdfs:domain <https://w3id.org/arco/ontology/context-description/RelatedWorkSituation> ;
                         rdfs:range [ rdf:type rdfs:Datatype ;
                                      owl:unionOf ( rdfs:Literal
                                                    xsd:int
                                                  )
                                    ] ;
                         rdfs:comment "Alternative date of a relation" .


###  https://github.com/MattiaSpadoni/LastSupper/blob/main/LastSupper.owl#ApproximateDate
:ApproximateDate rdf:type owl:DatatypeProperty ;
                 rdfs:subPropertyOf <https://w3id.org/italia/onto/TI/date> ;
                 rdfs:domain owl:Thing ;
                 rdfs:range rdfs:Literal ;
                 owl:propertyDisjointWith :EndDate ,
                                          :StartDate ;
                 rdfs:comment "Approximate date of an owl:thing" .


###  https://github.com/MattiaSpadoni/LastSupper/blob/main/LastSupper.owl#ApproximatePeriod
:ApproximatePeriod rdf:type owl:DatatypeProperty ;
                   rdfs:subPropertyOf :ApproximateDate ;
                   rdfs:domain owl:Thing ;
                   rdfs:range rdfs:Literal ;
                   rdfs:comment "Approximate period of an owl:thing" .


###  https://github.com/MattiaSpadoni/LastSupper/blob/main/LastSupper.owl#CompositionDescription
:CompositionDescription rdf:type owl:DatatypeProperty ;
                        rdfs:subPropertyOf :LongDescription ;
                        rdfs:domain owl:Thing ;
                        rdfs:range rdfs:Literal ;
                        owl:propertyDisjointWith :CompositionRelationDescription ;
                        rdfs:comment "Description of composition element of a owl:thing" .


###  https://github.com/MattiaSpadoni/LastSupper/blob/main/LastSupper.owl#CompositionRelationDescription
:CompositionRelationDescription rdf:type owl:DatatypeProperty ;
                                rdfs:subPropertyOf :RelationDescription ;
                                rdfs:domain <https://w3id.org/arco/ontology/context-description/RelatedWorkSituation> ;
                                rdfs:range rdfs:Literal ;
                                rdfs:comment "Property describing the influence a work has on another from a composition point of view. Eg: Marcantonio Raimondi Last Supper shows a composition influenced by the symmetry and the groupings of 3 of Leonardo Last Supper" .


###  https://github.com/MattiaSpadoni/LastSupper/blob/main/LastSupper.owl#Description
:Description rdf:type owl:DatatypeProperty ;
             rdfs:domain owl:Thing ;
             rdfs:range rdfs:Literal ;
             rdfs:comment "Long textual description of an owl thing." .


###  https://github.com/MattiaSpadoni/LastSupper/blob/main/LastSupper.owl#EndDate
:EndDate rdf:type owl:DatatypeProperty ;
         rdfs:subPropertyOf <https://w3id.org/italia/onto/TI/date> ;
         rdfs:domain owl:Thing ;
         rdfs:range rdfs:Literal ;
         rdfs:comment "End date of an owl:thing" .


###  https://github.com/MattiaSpadoni/LastSupper/blob/main/LastSupper.owl#GeometricalDescription
:GeometricalDescription rdf:type owl:DatatypeProperty ;
                        rdfs:subPropertyOf :LongDescription ;
                        rdfs:domain owl:Thing ;
                        rdfs:range rdfs:Literal ;
                        owl:propertyDisjointWith :GeometricalRelationDescription ;
                        rdfs:comment "Description of geometric features of an owl:thing" .


###  https://github.com/MattiaSpadoni/LastSupper/blob/main/LastSupper.owl#GeometricalRelationDescription
:GeometricalRelationDescription rdf:type owl:DatatypeProperty ;
                                rdfs:subPropertyOf :RelationDescription ;
                                rdfs:domain <https://w3id.org/arco/ontology/context-description/RelatedWorkSituation> ;
                                rdfs:range rdfs:Literal ;
                                rdfs:comment "Property describing the geometrical influence a work has on another from a Geometrical point of view. Eg: The symmetry used in Leonardo Last Supper partially reused in Albrecht Durer Last Supper of 1523" .


###  https://github.com/MattiaSpadoni/LastSupper/blob/main/LastSupper.owl#Label
:Label rdf:type owl:DatatypeProperty ;
       rdfs:domain owl:Thing ;
       rdfs:range rdfs:Literal ;
       rdfs:isDefinedBy rdfs:label .


###  https://github.com/MattiaSpadoni/LastSupper/blob/main/LastSupper.owl#LongDescription
:LongDescription rdf:type owl:DatatypeProperty ;
                 rdfs:subPropertyOf :Description ;
                 rdfs:domain owl:Thing ;
                 rdfs:range rdfs:Literal ;
                 rdfs:comment "Extensive description of an owl:thing" .


###  https://github.com/MattiaSpadoni/LastSupper/blob/main/LastSupper.owl#OtherIconclassCode
:OtherIconclassCode rdf:type owl:DatatypeProperty ;
                    rdfs:subPropertyOf <https://w3id.org/arco/ontology/context-description/iconclassCode> ;
                    rdfs:domain :IconographicTheme ;
                    rdfs:range rdfs:Literal ;
                    rdfs:comment "Mention of other possible Iconclass Code of an Iconographi theme." .


###  https://github.com/MattiaSpadoni/LastSupper/blob/main/LastSupper.owl#RealisationPeriod
:RealisationPeriod rdf:type owl:DatatypeProperty ;
                   rdfs:subPropertyOf <https://w3id.org/italia/onto/TI/date> ;
                   rdfs:domain owl:Thing ;
                   rdfs:range rdfs:Literal ;
                   rdfs:comment "Generic period of realisation of an owl:thing." .


###  https://github.com/MattiaSpadoni/LastSupper/blob/main/LastSupper.owl#RelationDate
:RelationDate rdf:type owl:DatatypeProperty ;
              rdfs:subPropertyOf <https://w3id.org/italia/onto/TI/date> ;
              rdfs:domain <https://w3id.org/arco/ontology/context-description/RelatedWorkSituation> ;
              rdfs:range [ rdf:type rdfs:Datatype ;
                           owl:unionOf ( rdfs:Literal
                                         xsd:int
                                       )
                         ] ;
              rdfs:comment "Date of a relation" .


###  https://github.com/MattiaSpadoni/LastSupper/blob/main/LastSupper.owl#RelationDescription
:RelationDescription rdf:type owl:DatatypeProperty ;
                     rdfs:subPropertyOf :Description ;
                     rdfs:domain <https://w3id.org/arco/ontology/context-description/RelatedWorkSituation> ;
                     rdfs:range rdfs:Literal ;
                     rdfs:comment "Long description of a relation between 2 entities in a RelatedWorkSituation class." .


###  https://github.com/MattiaSpadoni/LastSupper/blob/main/LastSupper.owl#StartDate
:StartDate rdf:type owl:DatatypeProperty ;
           rdfs:subPropertyOf <https://w3id.org/italia/onto/TI/date> ;
           rdfs:domain owl:Thing ;
           rdfs:range rdfs:Literal ;
           rdfs:comment "Start date of an owl:thing" .


###  https://github.com/MattiaSpadoni/LastSupper/blob/main/LastSupper.owl#TypicalIconclassCode
:TypicalIconclassCode rdf:type owl:DatatypeProperty ;
                      rdfs:subPropertyOf <https://w3id.org/arco/ontology/context-description/iconclassCode> ;
                      rdfs:domain :IconographicTheme ;
                      rdfs:range rdfs:Literal ;
                      rdfs:comment "Mention of the typical Iconclass Code used to mark the episode of an iconographic theme." .


###  https://github.com/MattiaSpadoni/LastSupper/blob/main/LastSupper.owl#URI
:URI rdf:type owl:DatatypeProperty ;
     rdfs:range xsd:string ;
     rdfs:comment "This property gives the plain value of URI of the image file." .


###  https://w3id.org/arco/ontology/context-description/agentDate
<https://w3id.org/arco/ontology/context-description/agentDate> rdf:type owl:DatatypeProperty ;
                                                               rdfs:subPropertyOf <https://w3id.org/italia/onto/TI/date> ;
                                                               rdfs:domain <https://w3id.org/italia/onto/l0/Agent> ;
                                                               rdfs:range rdfs:Literal ;
                                                               rdfs:comment "This property allows you to associate generic chronological indications to an agent."^^rdfs:Literal ;
                                                               rdfs:isDefinedBy "https://w3id.org/arco/ontology/context-description/agentDate"^^rdfs:Literal .


###  https://w3id.org/arco/ontology/context-description/bibliographicReferenceAuthor
<https://w3id.org/arco/ontology/context-description/bibliographicReferenceAuthor> rdf:type owl:DatatypeProperty ;
                                                                                  rdfs:domain <https://w3id.org/arco/ontology/context-description/Bibliography> ;
                                                                                  rdfs:range rdfs:Literal ;
                                                                                  rdfs:comment "This property represents the author related to the bibliographic reference." .


###  https://w3id.org/arco/ontology/context-description/bilbiographicReference
<https://w3id.org/arco/ontology/context-description/bilbiographicReference> rdf:type owl:DatatypeProperty ;
                                                                            rdfs:domain <https://w3id.org/arco/ontology/context-description/Bibliography> ;
                                                                            rdfs:range rdfs:Literal ;
                                                                            rdfs:comment "This property represents the bibliographic reference." .


###  https://w3id.org/arco/ontology/context-description/iconclassCode
<https://w3id.org/arco/ontology/context-description/iconclassCode> rdf:type owl:DatatypeProperty ;
                                                                   rdfs:domain :IconographicTheme ;
                                                                   rdfs:range rdfs:Literal ;
                                                                   rdfs:comment "This property represents the Iconclass code, for describing the subject or ornamental motif represented by the cultural property." ;
                                                                   rdfs:isDefinedBy <https://w3id.org/arco/ontology/context-description/iconclassCode> .


###  https://w3id.org/italia/onto/CLV/coordinate
<https://w3id.org/italia/onto/CLV/coordinate> rdf:type owl:DatatypeProperty ;
                                              rdfs:domain <https://w3id.org/italia/onto/CLV/Geometry> ;
                                              rdfs:range rdfs:Literal ;
                                              rdfs:comment "This property represents the geographical coordinate of the Geometry" .


###  https://w3id.org/italia/onto/CLV/lat
<https://w3id.org/italia/onto/CLV/lat> rdf:type owl:DatatypeProperty ;
                                       rdfs:subPropertyOf <https://w3id.org/italia/onto/CLV/coordinate> ;
                                       rdfs:domain <https://w3id.org/italia/onto/CLV/Geometry> ;
                                       rdfs:range rdfs:Literal ;
                                       rdfs:comment "This property represents the latitude. It is associated with the Geometry." .


###  https://w3id.org/italia/onto/CLV/long
<https://w3id.org/italia/onto/CLV/long> rdf:type owl:DatatypeProperty ;
                                        rdfs:subPropertyOf <https://w3id.org/italia/onto/CLV/coordinate> ;
                                        rdfs:domain <https://w3id.org/italia/onto/CLV/Geometry> ;
                                        rdfs:range rdfs:Literal ;
                                        rdfs:comment "This property allows one to specify the longitude. It is associated with the Geometry" .


###  https://w3id.org/italia/onto/TI/date
<https://w3id.org/italia/onto/TI/date> rdf:type owl:DatatypeProperty ;
                                       rdfs:domain owl:Thing ;
                                       rdfs:range [ rdf:type rdfs:Datatype ;
                                                    owl:unionOf ( rdfs:Literal
                                                                  xsd:int
                                                                )
                                                  ] ;
                                       rdfs:comment "This property represents a generic date / time instant." ;
                                       rdfs:isDefinedBy <https://w3id.org/italia/onto/TI/date> .


###  https://w3id.org/italia/onto/l0/name
<https://w3id.org/italia/onto/l0/name> rdf:type owl:DatatypeProperty ;
                                       rdfs:domain owl:Thing ;
                                       rdfs:range rdfs:Literal .


#################################################################
#    Classes
#################################################################

###  http://dati.beniculturali.it/cis/CulturalEntity
<http://dati.beniculturali.it/cis/CulturalEntity> rdf:type owl:Class ;
                                                  rdfs:comment "Class that provides a generalization of three classes; that is , cultural institute or site, collection and cultural heritage object. It does not correspond to a concept used typically in the cultural domain but it is used in order to model properties and property restrictions that are common to all the these three classes. The class will never be directly instanziated."@en .


###  http://xmlns.com/foaf/0.1/Image
<http://xmlns.com/foaf/0.1/Image> rdf:type owl:Class ;
                                  rdfs:comment """The class Image is a sub-class of Document corresponding to those documents which are images.
Digital images (such as JPEG, PNG, GIF bitmaps, SVG diagrams etc.) are examples of Image."""@en .


###  https://github.com/MattiaSpadoni/LastSupper/blob/main/LastSupper.owl#AbstractConcept
:AbstractConcept rdf:type owl:Class ;
                 rdfs:subClassOf <https://w3id.org/italia/onto/l0/Concept> ;
                 rdfs:comment "This class represent a specification class for the \"Concept\". It is not thought to be directly instatiated, but only to be a collector of more defined abstract concepts as artistic theories and iconographies"^^rdfs:Literal .


###  https://github.com/MattiaSpadoni/LastSupper/blob/main/LastSupper.owl#ArtisticTheory
:ArtisticTheory rdf:type owl:Class ;
                rdfs:subClassOf :AbstractConcept ;
                rdfs:comment """This class collects artistic theories, they are what an author/artist thinks the art practice should be and what they want to represent. An artistic theories does not necessarily have strict rules and it does not need to be consciously defined.
E.g. Leonardo's Teoria dei moti dell'animo is an artistic theory, there are literary sources talking about it but Leonardo did not identified strict rules nor defined a clear definition for it."""^^rdfs:Literal .


###  https://github.com/MattiaSpadoni/LastSupper/blob/main/LastSupper.owl#Character
:Character rdf:type owl:Class ;
           rdfs:subClassOf :PictorialAttribute ;
           rdfs:comment "A character is a figure playing a certain role inside a representation. It is indipendent from the representation itself. E.g. S. Peter is a character of Last Supper iconography." .


###  https://github.com/MattiaSpadoni/LastSupper/blob/main/LastSupper.owl#CompositionMotif
:CompositionMotif rdf:type owl:Class ;
                  rdfs:subClassOf :VisualUnit ;
                  owl:disjointWith :GeometricVisualUnit ;
                  rdfs:comment "Specialisation of VisualUnit, it represent VisualUnit identified to be representative of composition elements of a painting. Eg: the groupings of 3 figures in Last Supper." .


###  https://github.com/MattiaSpadoni/LastSupper/blob/main/LastSupper.owl#DerivationRelation
:DerivationRelation rdf:type owl:Class ;
                    rdfs:subClassOf <https://w3id.org/arco/ontology/context-description/RelatedWorkSituation> ;
                    rdfs:comment "This class is a specialisation of a RelatedWorkSituation one. It aims to represent a special type of relation that is the derivation relation among 2 different cultural properties."@en .


###  https://github.com/MattiaSpadoni/LastSupper/blob/main/LastSupper.owl#GeometricVisualUnit
:GeometricVisualUnit rdf:type owl:Class ;
                     rdfs:subClassOf :VisualUnit ;
                     rdfs:comment "Specialisation of VisualUnit. It comprise visualUnit aimed at showing the geometrical elements of a painting. Eg: the perspective lines of Last Supper" .


###  https://github.com/MattiaSpadoni/LastSupper/blob/main/LastSupper.owl#IconographicTheme
:IconographicTheme rdf:type owl:Class ;
                   rdfs:subClassOf :AbstractConcept ;
                   rdfs:comment "This class is a general collector of all iconographies sharing the same theme. Eg. All Last Supper iconographies are connected to the instance of Iconographic Theme \"Last Supper\". It serves as a general overview of registered iconographies."^^rdfs:Literal .


###  https://github.com/MattiaSpadoni/LastSupper/blob/main/LastSupper.owl#Iconography
:Iconography rdf:type owl:Class ;
             rdfs:subClassOf :AbstractConcept ;
             rdfs:comment "This class is the single iconographical representation. Each instance of this class could be present in different cultural properties and has a specific set of features that distinguish it from another one. Example: Florentine Last Supper is a way of representing Last Supper with certain temporal and location characteristics and with specific visual features."^^rdfs:Literal .


###  https://github.com/MattiaSpadoni/LastSupper/blob/main/LastSupper.owl#InfluenceRelation
:InfluenceRelation rdf:type owl:Class ;
                   rdfs:subClassOf <https://w3id.org/arco/ontology/context-description/RelatedWorkSituation> ;
                   rdfs:comment "This class represent the influence relation between two cultural properties. One artwork influencing in every possible way another one establish an InfluenceRelation."@en .


###  https://github.com/MattiaSpadoni/LastSupper/blob/main/LastSupper.owl#PictorialAttribute
:PictorialAttribute rdf:type owl:Class ;
                    rdfs:comment "It is a significant element of an iconographical representation. it difference itself from a simple visual features due to its having an indipendence from the representation itself. Example: Last Supper has inside it the figure of Peter. Peter is a character that is independent from a single painting."^^rdfs:Literal .


###  https://github.com/MattiaSpadoni/LastSupper/blob/main/LastSupper.owl#PreparatoryRelation
:PreparatoryRelation rdf:type owl:Class ;
                     rdfs:subClassOf <https://w3id.org/arco/ontology/context-description/RelatedWorkSituation> ;
                     rdfs:comment "This class is the one responsible for representing the preparatory relation between two cultural properties, the preparatory and the final one. Eg: Windsor 12542 being a preparatory work of Last Supper"@en .


###  https://github.com/MattiaSpadoni/LastSupper/blob/main/LastSupper.owl#SceneObject
:SceneObject rdf:type owl:Class ;
             rdfs:subClassOf :PictorialAttribute ;
             rdfs:comment "A scene object is a significant object existing inside an artwork. It is different from pure shapes and arrangements of motif due to fact that it could be represented in many differet ways but it is always present in certain representation. For example the figure of S. Peter in Last Supper always have a knife." .


###  https://github.com/MattiaSpadoni/LastSupper/blob/main/LastSupper.owl#VisualUnit
:VisualUnit rdf:type owl:Class ;
            rdfs:subClassOf <http://xmlns.com/foaf/0.1/Image> ;
            rdfs:comment "This class represent significant visive units coming from an artwork. It has no proper meaning besides being images. The image of this class is the little as possible detail."@en .


###  https://w3id.org/arco/ontology/arco/CulturalProperty
<https://w3id.org/arco/ontology/arco/CulturalProperty> rdf:type owl:Class ;
                                                       rdfs:subClassOf <http://dati.beniculturali.it/cis/CulturalEntity> ;
                                                       rdfs:comment "This class represents a cultural property, both tangible and intangible. A cultural property is the legacy, tangible or intangible, recognised as part of the national cultural heritage, since it helps know and reconstruct the history and the landscape."@en ;
                                                       rdfs:isDefinedBy <https://w3id.org/arco/ontology/arco/CulturalProperty> .


###  https://w3id.org/arco/ontology/context-description/AlternativeDating
<https://w3id.org/arco/ontology/context-description/AlternativeDating> rdf:type owl:Class ;
                                                                       rdfs:subClassOf <https://w3id.org/arco/ontology/context-description/Dating> ;
                                                                       rdfs:comment "This class represents an alternative dating of a cultural property (e.g.: an obsolete dating, a dating based on another method of dating)."@en ;
                                                                       rdfs:isDefinedBy <https://w3id.org/arco/ontology/context-description/AlternativeDating> .


###  https://w3id.org/arco/ontology/context-description/Bibliography
<https://w3id.org/arco/ontology/context-description/Bibliography> rdf:type owl:Class ;
                                                                  rdfs:comment "Questa classe rappresenta un riferimento bibliografico che riguarda un'entità, per esempio un bene culturale." .


###  https://w3id.org/arco/ontology/context-description/BibliographyType
<https://w3id.org/arco/ontology/context-description/BibliographyType> rdf:type owl:Class ;
                                                                      rdfs:comment "Questa classe rappresenta il tipo di riferimento bibliografico." .


###  https://w3id.org/arco/ontology/context-description/CulturalPropertyStage
<https://w3id.org/arco/ontology/context-description/CulturalPropertyStage> rdf:type owl:Class ;
                                                                           rdfs:subClassOf <https://w3id.org/arco/ontology/core/CulturalEntityCharacteristic> ;
                                                                           rdfs:comment "This class represents the stage of the catalogued cultural property related to the object which constitutes its preparatory or final stage."@en ;
                                                                           rdfs:isDefinedBy <https://w3id.org/arco/ontology/context-description/CulturalPropertyStage> .


###  https://w3id.org/arco/ontology/context-description/Dating
<https://w3id.org/arco/ontology/context-description/Dating> rdf:type owl:Class ;
                                                            rdfs:subClassOf <https://w3id.org/arco/ontology/context-description/DetectionMethod> ,
                                                                            <https://w3id.org/arco/ontology/context-description/Interpretation> ;
                                                            rdfs:comment "This class represents the dating of an entity, that is information about the chronology of the entity (e.g.: a cultural property), referring to a particular event (e.g.: the creation of the cultural property, its distruction, etc.)"@en ;
                                                            rdfs:isDefinedBy <https://w3id.org/arco/ontology/context-description/Dating> .


###  https://w3id.org/arco/ontology/context-description/DetectionMethod
<https://w3id.org/arco/ontology/context-description/DetectionMethod> rdf:type owl:Class ;
                                                                     rdfs:subClassOf <https://w3id.org/arco/ontology/core/Method> ;
                                                                     rdfs:comment "This class represents the method of detection that allowed the detection of a cultural property and which is indicative of the type and consistency of some information in the catalogue record that describes it (e.g.: coring, archive data, oral sources)." .


###  https://w3id.org/arco/ontology/context-description/Interpretation
<https://w3id.org/arco/ontology/context-description/Interpretation> rdf:type owl:Class ;
                                                                    rdfs:subClassOf <https://w3id.org/arco/ontology/core/Situation> ;
                                                                    rdfs:comment "This class represents a situation in which pieces of information related to an object (e.g.: a cultural property) are detected and recorded by an agent, based on a specific source or motivation (e.g.:ithe authorship attribution, commission, etc.)"@en .


###  https://w3id.org/arco/ontology/context-description/InterpretationCriterion
<https://w3id.org/arco/ontology/context-description/InterpretationCriterion> rdf:type owl:Class ;
                                                                             rdfs:subClassOf <https://w3id.org/italia/onto/l0/Description> ;
                                                                             rdfs:comment "This class represents the criterion that motivated an interpretation (e.g. inscription, bibliography, documentation)." ;
                                                                             rdfs:isDefinedBy <https://w3id.org/arco/ontology/context-description/InterpretationCriterion> .


###  https://w3id.org/arco/ontology/context-description/RelatedWorkSituation
<https://w3id.org/arco/ontology/context-description/RelatedWorkSituation> rdf:type owl:Class ;
                                                                          rdfs:subClassOf <https://w3id.org/arco/ontology/core/Situation> ;
                                                                          rdfs:comment "This class represents a situation in which a cultural property is related to another work, that could even be another cultural property. The cultural property stage is defined referring to this relationship with a related work, that can represent a preparatory, a final phase or a derivation of the cultural property. When the relationship is between two cultural properties, when possible, the nature of the relationship is specified (e.g.: finding location)"@en ;
                                                                          rdfs:isDefinedBy <https://w3id.org/arco/ontology/context-description/RelatedWorkSituation> .


###  https://w3id.org/arco/ontology/context-description/Subject
<https://w3id.org/arco/ontology/context-description/Subject> rdf:type owl:Class ;
                                                             rdfs:subClassOf <https://w3id.org/italia/onto/l0/Topic> ;
                                                             rdfs:comment "This class represents the subject of a cultural property, or its ornamental motif." ;
                                                             rdfs:isDefinedBy <https://w3id.org/arco/ontology/context-description/Subject> .


###  https://w3id.org/arco/ontology/context-description/hasCulturalScope
<https://w3id.org/arco/ontology/context-description/hasCulturalScope> rdf:type owl:Class ;
                                                                      rdfs:subClassOf <https://w3id.org/italia/onto/l0/Topic> ;
                                                                      rdfs:comment "This property relates a situation, where a cultural scope is attributed to a cultural entity, to the cultural scope." ;
                                                                      rdfs:isDefinedBy <https://w3id.org/arco/ontology/context-description/CulturalScope> .


###  https://w3id.org/arco/ontology/core/CulturalEntityCharacteristic
<https://w3id.org/arco/ontology/core/CulturalEntityCharacteristic> rdf:type owl:Class ;
                                                                   rdfs:subClassOf <https://w3id.org/italia/onto/l0/Characteristic> ;
                                                                   rdfs:comment "The class representing the characteristic of a cultural entity (e.g. a cultural property)."@en .


###  https://w3id.org/arco/ontology/core/Method
<https://w3id.org/arco/ontology/core/Method> rdf:type owl:Class ;
                                             rdfs:subClassOf <https://w3id.org/italia/onto/l0/Description> ;
                                             rdfs:comment "The class representing the concept of method." .


###  https://w3id.org/arco/ontology/core/Situation
<https://w3id.org/arco/ontology/core/Situation> rdf:type owl:Class ;
                                                rdfs:subClassOf <https://w3id.org/italia/onto/l0/EventOrSituation> ;
                                                rdfs:comment "The class representing the generic concept of situation."@en .


###  https://w3id.org/italia/onto/CLV/Feature
<https://w3id.org/italia/onto/CLV/Feature> rdf:type owl:Class ;
                                           rdfs:subClassOf <https://w3id.org/italia/onto/CLV/SpatialObject> ;
                                           rdfs:comment "This class is used to represent any geographical entity." ;
                                           rdfs:isDefinedBy "https://w3id.org/italia/onto/CLV/Feature" .


###  https://w3id.org/italia/onto/CLV/Geometry
<https://w3id.org/italia/onto/CLV/Geometry> rdf:type owl:Class ;
                                            rdfs:subClassOf <https://w3id.org/italia/onto/CLV/SpatialObject> ;
                                            rdfs:comment "This class represents the geometry of a spatial entity." .


###  https://w3id.org/italia/onto/CLV/SpatialObject
<https://w3id.org/italia/onto/CLV/SpatialObject> rdf:type owl:Class ;
                                                 rdfs:subClassOf <https://w3id.org/italia/onto/l0/Location> ;
                                                 rdfs:comment "This class represents everything that can have a spatial representation." ;
                                                 rdfs:isDefinedBy "https://w3id.org/italia/onto/CLV/SpatialObject" .


###  https://w3id.org/italia/onto/TI/TemporalEntity
<https://w3id.org/italia/onto/TI/TemporalEntity> rdf:type owl:Class ;
                                                 rdfs:subClassOf <https://w3id.org/italia/onto/l0/Entity> ;
                                                 rdfs:comment "This class represents a temporal entity." .


###  https://w3id.org/italia/onto/TI/TimeInterval
<https://w3id.org/italia/onto/TI/TimeInterval> rdf:type owl:Class ;
                                               rdfs:subClassOf <https://w3id.org/italia/onto/TI/TemporalEntity> ,
                                                               <https://w3id.org/italia/onto/l0/Characteristic> ;
                                               rdfs:comment "A time interval"@en ,
                                                            "https://w3id.org/italia/onto/TI/TimeInterval"@en .


###  https://w3id.org/italia/onto/l0/Agent
<https://w3id.org/italia/onto/l0/Agent> rdf:type owl:Class ;
                                        rdfs:comment "Any agentive Object , either physical (e.g. a person, a robot, an oak), or social (e.g. a corporation, an institution, a community)."@en .


###  https://w3id.org/italia/onto/l0/Characteristic
<https://w3id.org/italia/onto/l0/Characteristic> rdf:type owl:Class ;
                                                 rdfs:subClassOf <https://w3id.org/italia/onto/l0/Entity> ;
                                                 rdfs:comment "The class of characteristics, intended as any aspect, attribuite, or quality of an entity. E.g. a certain size, aesthetic quality, color, etc."@en .


###  https://w3id.org/italia/onto/l0/Concept
<https://w3id.org/italia/onto/l0/Concept> rdf:type owl:Class ;
                                          rdfs:subClassOf <https://w3id.org/italia/onto/l0/Object> ;
                                          rdfs:comment "It is an object that is defined in some description. Once defined it can be used in other descriptions" ;
                                          rdfs:isDefinedBy <https://w3id.org/italia/onto/l0/Concept> .


###  https://w3id.org/italia/onto/l0/Description
<https://w3id.org/italia/onto/l0/Description> rdf:type owl:Class ;
                                              rdfs:subClassOf <https://w3id.org/italia/onto/l0/Object> ;
                                              rdfs:comment "The class of socially-created objects (texts, values, categories, relations, contexts) used to describe something else in a structured way. Examples include plans (as structured descriptions of actions to be executed), diagnoses (as structured descriptions of observed situations, explanations (as structured texts clarifying e.g. a concept), objective observations (as structured sets of values that identify a relevant situation)." .


###  https://w3id.org/italia/onto/l0/Entity
<https://w3id.org/italia/onto/l0/Entity> rdf:type owl:Class ;
                                         rdfs:comment "Anything: real, possible, or imaginary, which some modeller wants to talk about for some purpose."@en .


###  https://w3id.org/italia/onto/l0/EventOrSituation
<https://w3id.org/italia/onto/l0/EventOrSituation> rdf:type owl:Class ;
                                                   rdfs:subClassOf <https://w3id.org/italia/onto/l0/Entity> ;
                                                   rdfs:comment """This class represents a specific situation or an event that happens in the lifecycle of either a business or a person or a group of persons. The class is recommended.
Any entity that typically flows in time, either in the physical or social world Examples include athmospheric phenomena, concerts, travels, institutional processes, etc. It also represents a relational context created by an observer on the basis of a frame' Events are opposable to objects, since events typically flow in time, aggregating multiple objects during their flow, while objects tend to be stable in a certain time interval."""@en .


###  https://w3id.org/italia/onto/l0/Location
<https://w3id.org/italia/onto/l0/Location> rdf:type owl:Class ;
                                           rdfs:subClassOf <https://w3id.org/italia/onto/l0/Entity> ;
                                           rdfs:comment "The class including locations. Individuals of this class can be anything that is intended as a location for something else, e.g. geographical places, spatial objects, containers, etc." ;
                                           rdfs:isDefinedBy "https://w3id.org/italia/onto/l0/Location" .


###  https://w3id.org/italia/onto/l0/Object
<https://w3id.org/italia/onto/l0/Object> rdf:type owl:Class ;
                                         rdfs:subClassOf <https://w3id.org/italia/onto/l0/Entity> ;
                                         rdfs:comment "Any entity that tends to be stable in time, either in the physical or social world. Examples include homes, cities, organizations, works of art, natural objects, artifacts, words, ideas, etc. Objects are opposable to events, since events typically flow in time, aggregating multiple objects during their flow, as with working, travelling or leisure activities, industrial or athmospheric processes, etc." .


###  https://w3id.org/italia/onto/l0/Topic
<https://w3id.org/italia/onto/l0/Topic> rdf:type owl:Class ;
                                        rdfs:subClassOf <https://w3id.org/italia/onto/l0/Entity> ;
                                        rdfs:comment "The class of topics, subjects, arguments, categories, domains, etc., intended as topics of a discourse or a categorization." .


###  Generated by the OWL API (version 5.1.14) https://github.com/owlcs/owlapi/
